<?xml version="1.0" encoding="utf-8"?>
<rdf:RDF
  xmlns:owl="http://www.w3.org/2002/07/owl#"
  xmlns:rdf="http://www.w3.org/1999/02/22-rdf-syntax-ns#"
  xmlns:rdfs="http://www.w3.org/2000/01/rdf-schema#"
>
  <owl:Class rdf:about="https://cn.dataone.org/cn/v2/object/doi:10.5063/AA/bowdish.783.5#d_1_a_2">
    <rdfs:subClassOf rdf:resource="http://ecoinformatics.org/oboe/oboe.1.1/oboe-core.owl#MeasurementType"/>
    <rdfs:subClassOf>
      <owl:Restriction rdf:nodeID="N3942959e63a14cc7bcb699ec3b09cc6b">
        <owl:onProperty rdf:resource="http://ecoinformatics.org/oboe/oboe.1.1/oboe-core.owl#measuresCharacteristic"/>
        <owl:someValuesFrom rdf:resource="https://cn.dataone.org/cn/v2/object/doi:10.5063/AA/bowdish.783.5#d_1_c_2"/>
      </owl:Restriction>
    </rdfs:subClassOf>
    <rdfs:subClassOf>
      <owl:Restriction rdf:nodeID="N9872ca6e005a44ab9e57d5a9d066d516">
        <owl:someValuesFrom rdf:resource="https://cn.dataone.org/cn/v2/object/doi:10.5063/AA/bowdish.783.5#d_1"/>
        <owl:onProperty rdf:resource="http://ecoinformatics.org/oboe/oboe.1.1/oboe-core.owl#measuresEntity"/>
      </owl:Restriction>
    </rdfs:subClassOf>
    <rdfs:label>TableS1 Hedge's d</rdfs:label>
  </owl:Class>
  <owl:Class rdf:about="https://cn.dataone.org/cn/v2/object/doi:10.5063/AA/bowdish.783.5#d_1_a_6">
    <rdfs:subClassOf>
      <owl:Restriction rdf:nodeID="N543e0b5b70e74ea1a6f68041f9c694f2">
        <owl:onProperty rdf:resource="http://ecoinformatics.org/oboe/oboe.1.1/oboe-core.owl#measuresCharacteristic"/>
        <owl:someValuesFrom rdf:resource="https://cn.dataone.org/cn/v2/object/doi:10.5063/AA/bowdish.783.5#d_1_c_6"/>
      </owl:Restriction>
    </rdfs:subClassOf>
    <rdfs:label>TableS1 Hedge's d</rdfs:label>
    <rdfs:subClassOf rdf:resource="http://ecoinformatics.org/oboe/oboe.1.1/oboe-core.owl#MeasurementType"/>
    <rdfs:subClassOf>
      <owl:Restriction rdf:nodeID="Na6e599756dbf4eb2b9d950ecb30c834c">
        <owl:onProperty rdf:resource="http://ecoinformatics.org/oboe/oboe.1.1/oboe-core.owl#measuresEntity"/>
        <owl:someValuesFrom rdf:resource="https://cn.dataone.org/cn/v2/object/doi:10.5063/AA/bowdish.783.5#d_1"/>
      </owl:Restriction>
    </rdfs:subClassOf>
  </owl:Class>
  <owl:Class rdf:about="https://cn.dataone.org/cn/v2/object/doi:10.5063/AA/bowdish.783.5#d_1_a_9">
    <rdfs:label>TableS1 Hedge's d</rdfs:label>
    <rdfs:subClassOf>
      <owl:Restriction rdf:nodeID="N12821335eb994ec09d5d01236e770a24">
        <owl:someValuesFrom rdf:resource="https://cn.dataone.org/cn/v2/object/doi:10.5063/AA/bowdish.783.5#d_1_c_9"/>
        <owl:onProperty rdf:resource="http://ecoinformatics.org/oboe/oboe.1.1/oboe-core.owl#measuresCharacteristic"/>
      </owl:Restriction>
    </rdfs:subClassOf>
    <rdfs:subClassOf rdf:resource="http://ecoinformatics.org/oboe/oboe.1.1/oboe-core.owl#MeasurementType"/>
    <rdfs:subClassOf>
      <owl:Restriction rdf:nodeID="Ndb9f93b3300840bf82a82177ca04d1c2">
        <owl:someValuesFrom rdf:resource="https://cn.dataone.org/cn/v2/object/doi:10.5063/AA/bowdish.783.5#d_1"/>
        <owl:onProperty rdf:resource="http://ecoinformatics.org/oboe/oboe.1.1/oboe-core.owl#measuresEntity"/>
      </owl:Restriction>
    </rdfs:subClassOf>
  </owl:Class>
  <owl:Class rdf:about="https://cn.dataone.org/cn/v2/object/doi:10.5063/AA/bowdish.783.5#d_1_a_3">
    <rdfs:label>TableS1 Hedge's d</rdfs:label>
    <rdfs:subClassOf>
      <owl:Restriction rdf:nodeID="N1c151df0c03a457d82b4a42815ecb0c5">
        <owl:onProperty rdf:resource="http://ecoinformatics.org/oboe/oboe.1.1/oboe-core.owl#measuresEntity"/>
        <owl:someValuesFrom rdf:resource="https://cn.dataone.org/cn/v2/object/doi:10.5063/AA/bowdish.783.5#d_1"/>
      </owl:Restriction>
    </rdfs:subClassOf>
    <rdfs:subClassOf>
      <owl:Restriction rdf:nodeID="Ndc3c7218658542b4b5e43f086fc500e1">
        <owl:someValuesFrom rdf:resource="https://cn.dataone.org/cn/v2/object/doi:10.5063/AA/bowdish.783.5#d_1_c_3"/>
        <owl:onProperty rdf:resource="http://ecoinformatics.org/oboe/oboe.1.1/oboe-core.owl#measuresCharacteristic"/>
      </owl:Restriction>
    </rdfs:subClassOf>
    <rdfs:subClassOf rdf:resource="http://ecoinformatics.org/oboe/oboe.1.1/oboe-core.owl#MeasurementType"/>
  </owl:Class>
  <owl:Class rdf:about="https://cn.dataone.org/cn/v2/object/doi:10.5063/AA/bowdish.783.5#d_1_a_10">
    <rdfs:subClassOf>
      <owl:Restriction rdf:nodeID="N847227292b4c433097074680cb751be6">
        <owl:someValuesFrom rdf:resource="https://cn.dataone.org/cn/v2/object/doi:10.5063/AA/bowdish.783.5#d_1_c_10"/>
        <owl:onProperty rdf:resource="http://ecoinformatics.org/oboe/oboe.1.1/oboe-core.owl#measuresCharacteristic"/>
      </owl:Restriction>
    </rdfs:subClassOf>
    <rdfs:label>TableS1 Hedge's d</rdfs:label>
    <rdfs:subClassOf rdf:resource="http://ecoinformatics.org/oboe/oboe.1.1/oboe-core.owl#MeasurementType"/>
    <rdfs:subClassOf>
      <owl:Restriction rdf:nodeID="N02dd6edc1535414a99f4d5e0c91eeaee">
        <owl:onProperty rdf:resource="http://ecoinformatics.org/oboe/oboe.1.1/oboe-core.owl#measuresEntity"/>
        <owl:someValuesFrom rdf:resource="https://cn.dataone.org/cn/v2/object/doi:10.5063/AA/bowdish.783.5#d_1"/>
      </owl:Restriction>
    </rdfs:subClassOf>
  </owl:Class>
  <owl:Class rdf:about="https://cn.dataone.org/cn/v2/object/doi:10.5063/AA/bowdish.783.5#d_1_a_7">
    <rdfs:label>TableS1 Hedge's d</rdfs:label>
    <rdfs:subClassOf>
      <owl:Restriction rdf:nodeID="Nafa208d16c724fb39cf2d2c9754310d6">
        <owl:someValuesFrom rdf:resource="https://cn.dataone.org/cn/v2/object/doi:10.5063/AA/bowdish.783.5#d_1"/>
        <owl:onProperty rdf:resource="http://ecoinformatics.org/oboe/oboe.1.1/oboe-core.owl#measuresEntity"/>
      </owl:Restriction>
    </rdfs:subClassOf>
    <rdfs:subClassOf rdf:resource="http://ecoinformatics.org/oboe/oboe.1.1/oboe-core.owl#MeasurementType"/>
    <rdfs:subClassOf>
      <owl:Restriction rdf:nodeID="Nc36758c400e64552a5e378ed51b47e9e">
        <owl:onProperty rdf:resource="http://ecoinformatics.org/oboe/oboe.1.1/oboe-core.owl#measuresCharacteristic"/>
        <owl:someValuesFrom rdf:resource="https://cn.dataone.org/cn/v2/object/doi:10.5063/AA/bowdish.783.5#d_1_c_7"/>
      </owl:Restriction>
    </rdfs:subClassOf>
  </owl:Class>
  <owl:Class rdf:about="https://cn.dataone.org/cn/v2/object/doi:10.5063/AA/bowdish.783.5#d_1_a_4">
    <rdfs:label>TableS1 Hedge's d</rdfs:label>
    <rdfs:subClassOf rdf:resource="http://ecoinformatics.org/oboe/oboe.1.1/oboe-core.owl#MeasurementType"/>
    <rdfs:subClassOf>
      <owl:Restriction rdf:nodeID="N5f2b0644323644609a3830cbeba73cd1">
        <owl:onProperty rdf:resource="http://ecoinformatics.org/oboe/oboe.1.1/oboe-core.owl#measuresCharacteristic"/>
        <owl:someValuesFrom rdf:resource="https://cn.dataone.org/cn/v2/object/doi:10.5063/AA/bowdish.783.5#d_1_c_4"/>
      </owl:Restriction>
    </rdfs:subClassOf>
    <rdfs:subClassOf>
      <owl:Restriction rdf:nodeID="Nc9da69e6290543c89418c43beb890718">
        <owl:someValuesFrom rdf:resource="https://cn.dataone.org/cn/v2/object/doi:10.5063/AA/bowdish.783.5#d_1"/>
        <owl:onProperty rdf:resource="http://ecoinformatics.org/oboe/oboe.1.1/oboe-core.owl#measuresEntity"/>
      </owl:Restriction>
    </rdfs:subClassOf>
  </owl:Class>
  <owl:Class rdf:about="https://cn.dataone.org/cn/v2/object/doi:10.5063/AA/bowdish.783.5#d_1_a_5">
    <rdfs:subClassOf rdf:resource="http://ecoinformatics.org/oboe/oboe.1.1/oboe-core.owl#MeasurementType"/>
    <rdfs:subClassOf>
      <owl:Restriction rdf:nodeID="N8104b0ec4f504788b8aa8b3d94e286ce">
        <owl:onProperty rdf:resource="http://ecoinformatics.org/oboe/oboe.1.1/oboe-core.owl#measuresEntity"/>
        <owl:someValuesFrom rdf:resource="https://cn.dataone.org/cn/v2/object/doi:10.5063/AA/bowdish.783.5#d_1"/>
      </owl:Restriction>
    </rdfs:subClassOf>
    <rdfs:label>TableS1 Hedge's d</rdfs:label>
    <rdfs:subClassOf>
      <owl:Restriction rdf:nodeID="N00c0f433baaa46dfbe63347571dc0bc6">
        <owl:onProperty rdf:resource="http://ecoinformatics.org/oboe/oboe.1.1/oboe-core.owl#measuresCharacteristic"/>
        <owl:someValuesFrom rdf:resource="https://cn.dataone.org/cn/v2/object/doi:10.5063/AA/bowdish.783.5#d_1_c_5"/>
      </owl:Restriction>
    </rdfs:subClassOf>
  </owl:Class>
  <owl:Class rdf:about="https://cn.dataone.org/cn/v2/object/doi:10.5063/AA/bowdish.783.5#d_1_a_1">
    <rdfs:subClassOf>
      <owl:Restriction rdf:nodeID="N87c3436b18144004a5d54f83699d025c">
        <owl:onProperty rdf:resource="http://ecoinformatics.org/oboe/oboe.1.1/oboe-core.owl#measuresCharacteristic"/>
        <owl:someValuesFrom rdf:resource="https://cn.dataone.org/cn/v2/object/doi:10.5063/AA/bowdish.783.5#d_1_c_1"/>
      </owl:Restriction>
    </rdfs:subClassOf>
    <rdfs:subClassOf>
      <owl:Restriction rdf:nodeID="Na7eda705f7734167b754abf0f362ca79">
        <owl:onProperty rdf:resource="http://ecoinformatics.org/oboe/oboe.1.1/oboe-core.owl#measuresEntity"/>
        <owl:someValuesFrom rdf:resource="https://cn.dataone.org/cn/v2/object/doi:10.5063/AA/bowdish.783.5#d_1"/>
      </owl:Restriction>
    </rdfs:subClassOf>
    <rdfs:label>TableS1 Hedge's d</rdfs:label>
    <rdfs:subClassOf rdf:resource="http://ecoinformatics.org/oboe/oboe.1.1/oboe-core.owl#MeasurementType"/>
  </owl:Class>
  <owl:Ontology rdf:about="https://cn.dataone.org/cn/v2/object/doi:10.5063/AA/bowdish.783.5">
    <rdfs:comment>List of 89 plant species selected for the meta-analysis. For each species we show the botanical family, the value of effect size (Hedge's d) and its variance (Vd), the compatibility system (CS), pollination specialization (PS), life form (LF), habitat type, geographic region and the source publication where information was obtained. SI: self-incompatible, SC: self-compatible, S: specialist, G: generalist, T: tree, Sh: shrub, V: vine, H: herb, Hp: hemi-parasite, ep: epiphyte. ‡ (double dagger symbol) Species from which the effects of habitat fragmentation on the pollination process were also assessed and thus were evaluated in a separate meta-analysis (cf. Methods section). This table is part of the supplemntary material included with Ecology Letters, Ramiro Aguilar, Lorena Ashworth, Leonardo Galetto, Marcelo Adrián Aizen (2006), Plant reproductive susceptibility to habitat fragmentation: review and synthesis through a meta-analysis, Ecology Letters 9 (8), 968-980. doi:10.1111/j.1461-0248.2006.00927.x</rdfs:comment>
    <rdfs:label>Plant reproductive susceptibility to habitat fragmentation meta-analysis</rdfs:label>
  </owl:Ontology>
  <owl:Class rdf:about="https://cn.dataone.org/cn/v2/object/doi:10.5063/AA/bowdish.783.5#d_1_a_8">
    <rdfs:label>TableS1 Hedge's d</rdfs:label>
    <rdfs:subClassOf>
      <owl:Restriction rdf:nodeID="N62fd6afce32c461491e44b00a7314c45">
        <owl:onProperty rdf:resource="http://ecoinformatics.org/oboe/oboe.1.1/oboe-core.owl#measuresEntity"/>
        <owl:someValuesFrom rdf:resource="https://cn.dataone.org/cn/v2/object/doi:10.5063/AA/bowdish.783.5#d_1"/>
      </owl:Restriction>
    </rdfs:subClassOf>
    <rdfs:subClassOf>
      <owl:Restriction rdf:nodeID="Nbe81a955162e4ab1985d5aacedd39011">
        <owl:onProperty rdf:resource="http://ecoinformatics.org/oboe/oboe.1.1/oboe-core.owl#measuresCharacteristic"/>
        <owl:someValuesFrom rdf:resource="https://cn.dataone.org/cn/v2/object/doi:10.5063/AA/bowdish.783.5#d_1_c_8"/>
      </owl:Restriction>
    </rdfs:subClassOf>
    <rdfs:subClassOf rdf:resource="http://ecoinformatics.org/oboe/oboe.1.1/oboe-core.owl#MeasurementType"/>
  </owl:Class>
  <owl:Class rdf:about="https://cn.dataone.org/cn/v2/object/doi:10.5063/AA/bowdish.783.5#d_1_c_8">
    <rdfs:subClassOf rdf:resource="http://ecoinformatics.org/oboe/oboe.1.1/oboe-core.owl#Characteristic"/>
    <rdfs:comment>Species, ones with ‡   (double dagger symbol) are Species from which the effects of habitat fragmentation on the pollination process were also assessed and thus were evaluated in a separate meta-analysis</rdfs:comment>
    <rdfs:label>Hedge's d</rdfs:label>
  </owl:Class>
  <owl:Class rdf:about="https://cn.dataone.org/cn/v2/object/doi:10.5063/AA/bowdish.783.5#d_1_c_2">
    <rdfs:subClassOf rdf:resource="http://ecoinformatics.org/oboe/oboe.1.1/oboe-core.owl#Characteristic"/>
    <rdfs:label>Hedge's d</rdfs:label>
    <rdfs:comment>Species, ones with ‡   (double dagger symbol) are Species from which the effects of habitat fragmentation on the pollination process were also assessed and thus were evaluated in a separate meta-analysis</rdfs:comment>
  </owl:Class>
  <owl:Class rdf:about="https://cn.dataone.org/cn/v2/object/doi:10.5063/AA/bowdish.783.5#d_1_c_5">
    <rdfs:subClassOf rdf:resource="http://ecoinformatics.org/oboe/oboe.1.1/oboe-core.owl#Characteristic"/>
    <rdfs:label>Hedge's d</rdfs:label>
    <rdfs:comment>Species, ones with ‡   (double dagger symbol) are Species from which the effects of habitat fragmentation on the pollination process were also assessed and thus were evaluated in a separate meta-analysis</rdfs:comment>
  </owl:Class>
  <owl:Class rdf:about="https://cn.dataone.org/cn/v2/object/doi:10.5063/AA/bowdish.783.5#d_1_c_1">
    <rdfs:subClassOf rdf:resource="http://ecoinformatics.org/oboe/oboe.1.1/oboe-core.owl#Characteristic"/>
    <rdfs:comment>Species, ones with ‡   (double dagger symbol) are Species from which the effects of habitat fragmentation on the pollination process were also assessed and thus were evaluated in a separate meta-analysis</rdfs:comment>
    <rdfs:label>Hedge's d</rdfs:label>
  </owl:Class>
  <owl:Class rdf:about="https://cn.dataone.org/cn/v2/object/doi:10.5063/AA/bowdish.783.5#d_1_c_3">
    <rdfs:subClassOf rdf:resource="http://ecoinformatics.org/oboe/oboe.1.1/oboe-core.owl#Characteristic"/>
    <rdfs:label>Hedge's d</rdfs:label>
    <rdfs:comment>Species, ones with ‡   (double dagger symbol) are Species from which the effects of habitat fragmentation on the pollination process were also assessed and thus were evaluated in a separate meta-analysis</rdfs:comment>
  </owl:Class>
  <owl:Class rdf:about="https://cn.dataone.org/cn/v2/object/doi:10.5063/AA/bowdish.783.5#d_1_c_6">
    <rdfs:subClassOf rdf:resource="http://ecoinformatics.org/oboe/oboe.1.1/oboe-core.owl#Characteristic"/>
    <rdfs:label>Hedge's d</rdfs:label>
    <rdfs:comment>Species, ones with ‡   (double dagger symbol) are Species from which the effects of habitat fragmentation on the pollination process were also assessed and thus were evaluated in a separate meta-analysis</rdfs:comment>
  </owl:Class>
  <owl:Class rdf:about="https://cn.dataone.org/cn/v2/object/doi:10.5063/AA/bowdish.783.5#d_1_c_4">
    <rdfs:comment>Species, ones with ‡   (double dagger symbol) are Species from which the effects of habitat fragmentation on the pollination process were also assessed and thus were evaluated in a separate meta-analysis</rdfs:comment>
    <rdfs:label>Hedge's d</rdfs:label>
    <rdfs:subClassOf rdf:resource="http://ecoinformatics.org/oboe/oboe.1.1/oboe-core.owl#Characteristic"/>
  </owl:Class>
  <owl:Class rdf:about="https://cn.dataone.org/cn/v2/object/doi:10.5063/AA/bowdish.783.5#d_1">
    <rdfs:subClassOf rdf:resource="http://ecoinformatics.org/oboe/oboe.1.1/oboe-core.owl#Entity"/>
    <rdfs:label>TableS1</rdfs:label>
    <rdfs:comment>Plant reproductive susceptibility to habitat fragmentation meta-analysis</rdfs:comment>
  </owl:Class>
  <owl:Class rdf:about="https://cn.dataone.org/cn/v2/object/doi:10.5063/AA/bowdish.783.5#d_1_c_10">
    <rdfs:subClassOf rdf:resource="http://ecoinformatics.org/oboe/oboe.1.1/oboe-core.owl#Characteristic"/>
    <rdfs:comment>Species, ones with ‡   (double dagger symbol) are Species from which the effects of habitat fragmentation on the pollination process were also assessed and thus were evaluated in a separate meta-analysis</rdfs:comment>
    <rdfs:label>Hedge's d</rdfs:label>
  </owl:Class>
  <owl:Class rdf:about="https://cn.dataone.org/cn/v2/object/doi:10.5063/AA/bowdish.783.5#d_1_c_7">
    <rdfs:subClassOf rdf:resource="http://ecoinformatics.org/oboe/oboe.1.1/oboe-core.owl#Characteristic"/>
    <rdfs:comment>Species, ones with ‡   (double dagger symbol) are Species from which the effects of habitat fragmentation on the pollination process were also assessed and thus were evaluated in a separate meta-analysis</rdfs:comment>
    <rdfs:label>Hedge's d</rdfs:label>
  </owl:Class>
  <owl:Class rdf:about="https://cn.dataone.org/cn/v2/object/doi:10.5063/AA/bowdish.783.5#d_1_c_9">
    <rdfs:subClassOf rdf:resource="http://ecoinformatics.org/oboe/oboe.1.1/oboe-core.owl#Characteristic"/>
    <rdfs:label>Hedge's d</rdfs:label>
    <rdfs:comment>Species, ones with ‡   (double dagger symbol) are Species from which the effects of habitat fragmentation on the pollination process were also assessed and thus were evaluated in a separate meta-analysis</rdfs:comment>
  </owl:Class>
</rdf:RDF>
